Check typing and clocking in one pass
This is slightly more efficient than doing it in two passes, but more
importantly, it allows for more accurate locations in error messages.

ObcToClight/DataflowElab.v
@@ -39,7 +39,7 @@ Parameter cabsloc_of_astloc : astloc -> Cabs.cabsloc.
 Parameter cabs_floatinfo : Ast.floatInfo -> Cabs.floatInfo.
 
 Definition err_loc (loc: astloc) (m: errmsg) :=
-  MSG (string_of_astloc loc) :: MSG ": " :: m.  
+  MSG (string_of_astloc loc) :: MSG ":" :: m.  
 
 (* TODO: move elsewhere *)
 Instance clock_EqDec : EqDec clock eq.
@@ -243,81 +243,106 @@ Section ElabExpressions.
     | Tbool    => Tint Ctypes.IBool Ctypes.Signed
     end.
 
-  Fixpoint elab_lexp (ae: Ast.expression) : res lexp :=
+  Fixpoint elab_lexp (ae: Ast.expression) : res (lexp * clock) :=
     match ae with
-    | CONSTANT c loc => OK (Econst (elab_constant loc c))
+    | CONSTANT c loc => OK (Econst (elab_constant loc c), Cbase)
     | VARIABLE sx loc =>
       let x := ident_of_camlstring sx in
       do ty <- find_type loc x;
-      OK (Evar x ty)
+      do ck <- find_clock loc x;
+      OK (Evar x ty, ck)
     | WHEN ae' b sx loc =>
       let x := ident_of_camlstring sx in
       do ok <- assert_type loc x bool_type;
-      do e' <- elab_lexp ae';
-      OK (Ewhen e' x b)
+      do (e', eck) <- elab_lexp ae';
+      do xck <- find_clock loc x;
+      if eck ==b xck then OK (Ewhen e' x b, Con xck x b)
+      else Error (err_loc loc (MSG "badly clocked when: "
+                                   :: msg_of_clocks eck xck))
     | UNARY aop ae' loc =>
       let op := elab_unop aop in
-      do e' <- elab_lexp ae';
+      do (e', ck) <- elab_lexp ae';
       do ty' <- find_type_unop loc op (typeof e');
-      OK (Eunop op e' ty')
+      OK (Eunop op e' ty', ck)
     | CAST aty' ae' loc =>
       let ty' := elab_type loc aty' in
-      do e' <- elab_lexp ae';
-      OK (Eunop (CastOp ty') e' ty')
+      do (e', ck) <- elab_lexp ae';
+      OK (Eunop (CastOp ty') e' ty', ck)
     | BINARY aop ae1 ae2 loc =>
       let op := elab_binop aop in
-      do e1 <- elab_lexp ae1;
-      do e2 <- elab_lexp ae2;
+      do (e1, ck1) <- elab_lexp ae1;
+      do (e2, ck2) <- elab_lexp ae2;
       do ty' <- find_type_binop loc op (typeof e1) (typeof e2);
-      OK (Ebinop op e1 e2 ty')
+      if ck1 ==b ck2 then OK (Ebinop op e1 e2 ty', ck1)
+      else Error (err_loc loc (MSG "badly clocked operator: "
+                                   :: msg_of_clocks ck1 ck2))
     | _ => Error (err_loc (expression_loc ae) (msg "expression not normalized"))
     end.
 
-  Fixpoint elab_cexp (ae: Ast.expression) : res cexp :=
+  Fixpoint elab_cexp (ae: Ast.expression) : res (cexp * clock) :=
     match ae with
     | MERGE sx aet aef loc =>
       let x := ident_of_camlstring sx in
       do ok <- assert_type loc x bool_type;
-      do et <- elab_cexp aet;
-      do ef <- elab_cexp aef;
+      do ck <- find_clock loc x;
+      do (et, ckt) <- elab_cexp aet;
+      do (ef, ckf) <- elab_cexp aef;
       if typeofc et ==b typeofc ef
-      then OK (Emerge x et ef)
+      then if (ckt ==b (Con ck x true))
+           then if (ckf ==b (Con ck x false))
+                then OK (Emerge x et ef, ck)
+                else Error (err_loc loc (MSG "badly clocked merge false branch: "
+                                         :: msg_of_clocks (Con ck x false) ckf))
+           else Error (err_loc loc (MSG "badly clocked merge true branch: "
+                                        :: msg_of_clocks (Con ck x true) ckt))
       else Error (err_loc loc (msg "badly typed merge"))
     | IFTE ae aet aef loc =>
-      do e <- elab_lexp ae;
-      do et <- elab_cexp aet;
-      do ef <- elab_cexp aef;
+      do (e, ck) <- elab_lexp ae;
+      do (et, ckt) <- elab_cexp aet;
+      do (ef, ckf) <- elab_cexp aef;
       if (typeof e ==b bool_type) && (typeofc et ==b typeofc ef)
-      then OK (Eite e et ef)
+      then if (ckt ==b ck)
+           then if (ckf ==b ck)
+                then OK (Eite e et ef, ck)
+                else Error (err_loc loc (MSG "badly clocked ifte false branch: "
+                                             :: msg_of_clocks ck ckf))
+           else Error (err_loc loc (MSG "badly clocked ifte true branch: "
+                                        :: msg_of_clocks ck ckt))
       else Error (err_loc loc (msg "badly typed if/then/else"))
     | _ =>
-      do e <- elab_lexp ae;
-      OK (Eexp e)
-    end.
-
+      do (e, ck) <- elab_lexp ae;
+      OK (Eexp e, ck)
+    end.  
+  
   Definition assert_lexp_type (loc: astloc) (e: lexp) (ty: type) : res unit :=
     if typeof e ==b ty then OK tt
     else Error (err_loc loc (MSG "badly typed argument: "
                                  :: msg_of_types ty (typeof e))).
 
-  Fixpoint elab_lexps (loc: astloc) (aes: list expression) (tys: list type)
+  Fixpoint elab_lexps (loc: astloc) (ck': clock) (aes: list expression)
+                      (tys: list type)
     : res (list lexp) :=
     match aes, tys with
     | nil, nil => OK nil
     | ae::aes, ty::tys =>
-      do e <- elab_lexp ae;
-      do ok <- assert_lexp_type (expression_loc ae) e ty;
-      do es <- elab_lexps loc aes tys;
-      OK (e::es)
+      do (e, ck) <- elab_lexp ae;
+      if ck ==b ck'
+      then do ok <- assert_lexp_type (expression_loc ae) e ty;
+           do es <- elab_lexps loc ck' aes tys;
+           OK (e::es)
+      else Error (err_loc loc ((MSG "ill-clocked argument expression "
+                                    :: msg_of_clocks ck ck')))
     | _, _ => Error (err_loc loc (msg "wrong number of arguments"))
     end.
 
-  Fixpoint check_result_list (loc: astloc) (xs: list ident) (ys: list type)
-                                                                   : res PS.t :=
+  Fixpoint check_result_list (loc: astloc) (ck: clock)
+                                           (xs: list ident) (ys: list type)
+                                                                : res PS.t :=
     match xs, ys with
     | nil, nil => OK PS.empty
     | x::xs, y::ys => do ok <- assert_type loc x y;
-                      do others <- check_result_list loc xs ys;
+                      do ok <- assert_clock loc x ck;
+                      do others <- check_result_list loc ck xs ys;
                       if PS.mem x others
                       then Error (err_loc loc
                                           (msg "duplicate variable in pattern"))
@@ -336,28 +361,6 @@ Section ElabExpressions.
     | _ => Error (err_loc loc (msg "fbys only take (casted) constants at left."))
     end.
 
-  (* TODO: in the next version, these checks should be integrated into
-           elab_lexp so that we can give more precise locations in
-           error messages (and also avoid traversing the term twice). *)
-  Fixpoint clock_of_lexp (loc: astloc) (le: lexp) : res clock :=
-    match le with
-    | Econst c           => OK Cbase
-    | Evar x ty          => find_clock loc x
-    | Ewhen e x b        =>
-      do eck <- clock_of_lexp loc e;
-      do xck <- find_clock loc x;
-      if eck ==b xck then OK (Con xck x b)
-      else Error (err_loc loc (MSG "badly clocked when: "
-                                   :: msg_of_clocks eck xck))
-    | Eunop op e ty      => clock_of_lexp loc e
-    | Ebinop op e1 e2 ty =>
-      do ck1 <- clock_of_lexp loc e1;
-      do ck2 <- clock_of_lexp loc e2;
-      if ck1 ==b ck2 then OK ck1
-      else Error (err_loc loc (MSG "badly clocked operator: "
-                                   :: msg_of_clocks ck1 ck2))
-    end.
-
   Lemma find_clock_clk_var:
     forall loc x ck,
       find_clock loc x = OK ck ->
@@ -367,70 +370,45 @@ Section ElabExpressions.
     intros loc x ck Hfind.
     NamedDestructCases; auto using clk_var.
   Qed.
-  
-  Lemma clock_of_lexp_spec:
-    forall loc le ck,
-      clock_of_lexp loc le = OK ck ->
-      clk_lexp cenv le ck.
-  Proof.
-    induction le; simpl; intros ck HH;
-      repeat match goal with H:_ = OK _ |- _ => monadInv H end;
-      NamedDestructCases;
-      repeat match goal with
-             | H:(_ ==b _) = true |- _ =>
-               rewrite equiv_decb_equiv in H; rewrite H in *; clear H
-             | H:find_clock _ _ = OK _ |- _ =>
-               apply find_clock_clk_var in H
-             end;
-      auto using clk_lexp.
-  Qed.
 
-  Fixpoint clock_of_cexp (loc: astloc) (e: cexp) : res clock :=
-    match e with
-    | Emerge x e1 e2 =>
-      do ck <- find_clock loc x;
-      do ck1 <- clock_of_cexp loc e1;
-      do ck2 <- clock_of_cexp loc e2;
-      if (ck1 ==b (Con ck x true))
-      then if (ck2 ==b (Con ck x false))
-           then OK ck
-           else Error (err_loc loc (MSG "badly clocked merge false branch: "
-                                        :: msg_of_clocks (Con ck x false) ck2))
-      else Error (err_loc loc (MSG "badly clocked merge true branch: "
-                                   :: msg_of_clocks (Con ck x true) ck1))
-    | Eite e e1 e2 =>
-      do ck <- clock_of_lexp loc e;
-      do ck1 <- clock_of_cexp loc e1;
-      do ck2 <- clock_of_cexp loc e2;
-      if (ck1 ==b ck)
-      then if (ck2 ==b ck)
-           then OK ck
-           else Error (err_loc loc (MSG "badly clocked ifte false branch: "
-                                        :: msg_of_clocks ck ck2))
-      else Error (err_loc loc (MSG "badly clocked ifte true branch: "
-                                   :: msg_of_clocks ck ck1))
-    | Eexp e => clock_of_lexp loc e
+  Definition elab_equation (aeq: Ast.equation) : res equation :=
+    let '(sxs, ae, loc) := aeq in
+    do xs <- OK (map ident_of_camlstring sxs);
+    do x <- match xs with
+            | x::xs => OK x
+            | _ => Error (err_loc loc (msg "at least one output is required"))
+            end;
+    do ck <- find_clock loc x;
+    match ae with
+    | CALL sf aes loc =>
+      let f := ident_of_camlstring sf in
+      do (tysin, tysout) <- find_node_interface loc f;
+      do es <- elab_lexps loc ck aes tysin;
+      do ok <- check_result_list loc ck xs tysout;
+      OK (EqApp xs ck f es)
+           
+    | FBY ae0 ae loc =>
+      do v0 <- elab_constant_with_cast loc ae0;
+      let v0ty := type_const v0 in
+      do (e, eck) <- elab_lexp ae;
+      do ok <- assert_type loc x v0ty;
+      if typeof e ==b v0ty
+      then if eck ==b ck
+           then OK (EqFby x ck v0 e)
+           else Error (err_loc loc (MSG "ill-clocked fby expression for "
+                                        :: CTX x :: msg_of_clocks ck eck))
+      else Error (err_loc loc (MSG "ill-typed fby expression for "
+                                   :: CTX x :: msg_of_types v0ty (typeof e)))
+
+    | _ =>
+      do (e, eck) <- elab_cexp ae;
+      do ok <- assert_type loc x (typeofc e);
+      if eck ==b ck
+      then OK (EqDef x ck e)
+      else Error (err_loc loc (MSG "ill-clocked expression for "
+                                   :: CTX x :: msg_of_clocks ck eck))
     end.
   
-  Lemma clock_of_cexp_spec:
-    forall loc e ck,
-      clock_of_cexp loc e = OK ck ->
-      clk_cexp cenv e ck.
-  Proof.
-    induction e; simpl; intros ck HH;
-      repeat match goal with H:_ = OK _ |- _ => monadInv H end;
-      NamedDestructCases;
-      repeat match goal with
-             | H:(_ ==b _) = true |- _ =>
-               rewrite equiv_decb_equiv in H; rewrite H in *; clear H
-             | H:find_clock _ _ = OK _ |- _ =>
-               apply find_clock_clk_var in H
-             | H:clock_of_lexp _ _ = OK _ |- _ =>
-               apply clock_of_lexp_spec in H
-             end;
-      auto using clk_cexp.
-  Qed.
-
   Fixpoint assert_clocks (loc: astloc) (ck: clock) (ys: list ident)
     : res unit :=
     match ys with
@@ -439,7 +417,7 @@ Section ElabExpressions.
       do ok <- assert_clock loc y ck;
       assert_clocks loc ck ys
     end.
-
+  
   Lemma assert_clock_spec:
     forall loc x ck,
       assert_clock loc x ck = OK tt ->
@@ -464,94 +442,6 @@ Section ElabExpressions.
     apply IHxs in EQ0.
     constructor; eauto using assert_clock_spec.
   Qed.
-
-  Fixpoint assert_lexp_clocks (loc: astloc) (ck: clock) (es: list lexp)
-    : res unit :=
-    match es with
-    | nil => OK tt
-    | e::es =>
-      do ck' <- clock_of_lexp loc e;
-      if ck ==b ck'
-      then assert_lexp_clocks loc ck es
-      else Error (err_loc loc ((MSG "ill-clocked argument expression "
-                                    :: msg_of_clocks ck ck')))
-    end.
-
-  Lemma assert_lexp_clocks_spec:
-    forall loc ck es,
-      assert_lexp_clocks loc ck es = OK tt ->
-      Forall (fun e=> clk_lexp cenv e ck) es.
-  Proof.
-    induction es as [|e es]; intro HH; try apply Forall_nil.
-    simpl in HH. monadInv HH; NamedDestructCases.
-    rewrite equiv_decb_equiv in Heq; rewrite <-Heq in *.
-    constructor; eauto using clock_of_lexp_spec.
-  Qed.
-
-  Fixpoint check_clock (loc: astloc) (ck: clock) : res unit :=
-    match ck with
-    | Cbase => OK tt
-    | Con ck x b =>
-      do ok <- check_clock loc ck;
-      do xck <- find_clock loc x;
-      if xck ==b ck then OK tt
-      else Error (err_loc loc ((MSG "badly-formed clock "
-                                    :: msg_of_clocks xck ck)))
-    end.
-  
-  Lemma check_clock_spec:
-    forall loc ck,
-      check_clock loc ck = OK tt ->
-      clk_clock cenv ck.
-  Proof.
-    induction ck; simpl; intro HH; auto using clk_clock.
-    monadInv HH; NamedDestructCases.
-    apply find_clock_clk_var in EQ1.
-    rewrite equiv_decb_equiv in Heq. rewrite Heq in *.
-    destruct x. auto.
-  Qed.
-
-  Definition elab_equation (aeq: Ast.equation) : res equation :=
-    let '(sxs, ae, loc) := aeq in
-    do xs <- OK (map ident_of_camlstring sxs);
-    do x <- match xs with
-            | x::xs => OK x
-            | _ => Error (err_loc loc (msg "at least one output is required"))
-            end;
-    do ck <- find_clock loc x;
-    match ae with
-    | CALL sf aes loc =>
-      let f := ident_of_camlstring sf in
-      do (tysin, tysout) <- find_node_interface loc f;
-      do es <- elab_lexps loc aes tysin;
-      do ok <- check_result_list loc xs tysout;
-      do ok <- assert_lexp_clocks loc ck es;
-      do ok <- assert_clocks loc ck xs;
-      OK (EqApp xs ck f es)
-           
-    | FBY ae0 ae loc =>
-      do v0 <- elab_constant_with_cast loc ae0;
-      let v0ty := type_const v0 in
-      do e <- elab_lexp ae;
-      do ok <- assert_type loc x v0ty;
-      do eck <- clock_of_lexp loc e;
-      if typeof e ==b v0ty
-      then if eck ==b ck
-           then OK (EqFby x ck v0 e)
-           else Error (err_loc loc (MSG "ill-clocked fby expression for "
-                                        :: CTX x :: msg_of_clocks ck eck))
-      else Error (err_loc loc (MSG "ill-typed fby expression for "
-                                   :: CTX x :: msg_of_types v0ty (typeof e)))
-
-    | _ =>
-      do e <- elab_cexp ae;
-      do ok <- assert_type loc x (typeofc e);
-      do eck <- clock_of_cexp loc e;
-      if eck ==b ck
-      then OK (EqDef x ck e)
-      else Error (err_loc loc (MSG "ill-clocked expression for "
-                                   :: CTX x :: msg_of_clocks ck eck))
-    end.
 
   (** Properties *)
   
@@ -596,12 +486,13 @@ Section ElabExpressions.
   Qed.
 
   Lemma wt_elab_lexp:
-    forall ae e,
-      elab_lexp ae = OK e ->
+    forall ae e ck,
+      elab_lexp ae = OK (e, ck) ->
       wt_lexp (PM.elements env) e.
   Proof.
-    induction ae; intros e Helab; monadInv Helab; constructor;
-      eauto using find_type_In, assert_type_In.
+    induction ae; intros e ck Helab; monadInv Helab;
+      NamedDestructCases; try constructor; intros; subst;
+      eauto using wt_lexp, find_type_In, assert_type_In.
     - unfold find_type_unop in EQ1.
       rewrite type_unop'_correct in EQ1.
       now DestructCases.
@@ -609,77 +500,109 @@ Section ElabExpressions.
       match goal with H:match ?e with _ => _ end = _ |- _ =>
                       destruct e eqn:He; try discriminate; injection H end.
       intro; subst.
-      now rewrite type_binop'_correct in He.
+      rewrite type_binop'_correct in He.
+      eauto using wt_lexp.
     - now rewrite type_castop.
   Qed.
 
+  Lemma wc_elab_lexp:
+    forall ae e ck,
+      elab_lexp ae = OK (e, ck) ->
+      clk_lexp cenv e ck.
+  Proof.
+    induction ae; intros e ck Helab; monadInv Helab;
+      NamedDestructCases; try constructor; intros; subst;
+      repeat match goal with
+             | H:(_ ==b _) = true |- _ =>
+               rewrite equiv_decb_equiv in H; rewrite H in *; clear H
+             | H:find_clock _ _ = OK _ |- _ =>
+               apply find_clock_clk_var in H
+             end;
+      eauto using clk_lexp.
+  Qed.
+
   Lemma wt_elab_lexps:
-    forall loc aes tys es,
-      elab_lexps loc aes tys = OK es ->
+    forall loc ck aes tys es,
+      elab_lexps loc ck aes tys = OK es ->
       (Forall (wt_lexp (PM.elements env)) es
        /\ Forall2 (fun e ty=>typeof e = ty) es tys).
   Proof.
     induction aes; simpl; intros ** Helab; DestructCases; auto.
     monadInv Helab.
+    NamedDestructCases.
+    monadInv EQ0.
     apply wt_elab_lexp in EQ.
     specialize (IHaes _ _ EQ0); destruct IHaes.
     unfold assert_lexp_type in EQ1.
-    NamedDestructCases. rewrite equiv_decb_equiv in Heq.
+    NamedDestructCases. rewrite equiv_decb_equiv in Heq0.
     auto.
   Qed.
-  
+
+  Lemma wc_elab_lexps:
+    forall loc ck aes tys es,
+      elab_lexps loc ck aes tys = OK es ->
+      Forall (fun e=>clk_lexp cenv e ck) es.
+  Proof.
+    induction aes; simpl; intros ** Helab; DestructCases; auto.
+    monadInv Helab.
+    NamedDestructCases.
+    monadInv EQ0.
+    apply wc_elab_lexp in EQ.
+    rewrite equiv_decb_equiv in Heq; rewrite Heq in *.
+    eauto.
+  Qed.
+
   Lemma wt_elab_cexp:
-    forall ae e,
-      elab_cexp ae = OK e ->
+    forall ae e ck,
+      elab_cexp ae = OK (e, ck) ->
       wt_cexp (PM.elements env) e.
   Proof.
-    induction ae; intros e Helab.
-    - apply bind_inversion in Helab.
-      destruct Helab as (le & Helab & Hexp).
-      monadInv Hexp. eauto using wt_elab_lexp with dftyping.
-    - apply bind_inversion in Helab.
-      destruct Helab as (le & Helab & Hexp).
-      monadInv Hexp. eauto using wt_elab_lexp with dftyping.
-    - monadInv Helab.
-      specialize (IHae2 _ EQ1); clear EQ1.
-      specialize (IHae3 _ EQ0); clear EQ0.
+    induction ae; intros e ck Helab;
+      apply bind_inversion in Helab;
+      try (destruct Helab as ((le & ck') & Helab & Hexp);
+           monadInv Hexp);
+      eauto using wt_elab_lexp with dftyping.
+    - specialize (IHae2 _ _ EQ); clear EQ.
+      specialize (IHae3 _ _ EQ1); clear EQ1.
       NamedDestructCases.
       apply andb_prop in Heq; destruct Heq as (Hg1 & Hg2).
       rewrite equiv_decb_equiv in Hg1, Hg2.
+      intros; subst.
       eauto using wt_elab_lexp with dftyping.
-    - apply bind_inversion in Helab.
-      destruct Helab as (le & Helab & Hexp).
-      monadInv Hexp. eauto using wt_elab_lexp with dftyping.
-    - apply bind_inversion in Helab.
-      destruct Helab as (le & Helab & Hexp).
-      monadInv Hexp. eauto using wt_elab_lexp with dftyping.
-    - apply bind_inversion in Helab.
-      destruct Helab as (le & Helab & Hexp).
-      monadInv Hexp. eauto using wt_elab_lexp with dftyping.
-    - apply bind_inversion in Helab.
-      destruct Helab as (le & Helab & Hexp).
-      monadInv Hexp. eauto using wt_elab_lexp with dftyping.
-    - apply bind_inversion in Helab.
-      destruct Helab as (le & Helab & Hexp).
-      monadInv Hexp. eauto using wt_elab_lexp with dftyping.
-    - apply bind_inversion in Helab.
-      destruct Helab as (le & Helab & Hexp).
-      monadInv Hexp. eauto using wt_elab_lexp with dftyping.
-    - monadInv Helab.
-      specialize (IHae1 _ EQ1); clear EQ1.
-      specialize (IHae2 _ EQ0); clear EQ0.
-      NamedDestructCases.
+    - destruct Helab as (? & Haty & Helab).
+      monadInv Helab. NamedDestructCases.
+      specialize (IHae1 _ _ EQ1); clear EQ1.
+      specialize (IHae2 _ _ EQ0); clear EQ0.
       rewrite equiv_decb_equiv in Heq.
+      intro; subst.
       eauto using assert_type_In with dftyping.
   Qed.
 
+  Lemma wc_elab_cexp:
+    forall ae e ck,
+      elab_cexp ae = OK (e, ck) ->
+      clk_cexp cenv e ck.
+  Proof.
+    induction ae; simpl; intros e ck HH;
+      repeat match goal with H:_ = OK _ |- _ => monadInv H end;
+      NamedDestructCases; intros; subst;
+      repeat match goal with
+             | H:(_ ==b _) = true |- _ =>
+               rewrite equiv_decb_equiv in H; rewrite H in *; clear H
+             | H:find_clock _ _ = OK _ |- _ =>
+               apply find_clock_clk_var in H
+             end;
+      eauto using clk_cexp, clk_lexp, wc_elab_lexp.
+  Qed.
+
   Lemma check_result_list_Forall2:
-    forall loc xs txs s,
-      check_result_list loc xs txs = OK s ->
+    forall loc ck xs txs s,
+      check_result_list loc ck xs txs = OK s ->
       Forall2 (fun x tx => In (x, tx) (PM.elements env)) xs txs
       /\ (forall x, PS.In x s <-> In x xs)
-      /\ NoDup xs.
-  Proof.
+      /\ NoDup xs
+      /\ Forall (fun x=>clk_var cenv x ck) xs.
+    Proof.
     induction xs as [|x xs]; simpl.
     - repeat split; DestructCases; auto using NoDup_nil.
       now apply not_In_empty.
@@ -688,13 +611,14 @@ Section ElabExpressions.
       DestructCases.
       match goal with H:_ = OK _ |- _ => monadInv H end.
       NamedDestructCases.
-      apply IHxs in EQ1.
-      destruct EQ1 as (Hin & Hset & Hnodup).
+      apply IHxs in EQ0.
+      destruct EQ0 as (Hin & Hset & Hnodup & Hclk).
       apply mem_spec_false in Heq. rewrite Hset in Heq.
       apply assert_type_In in EQ.
-      repeat split; eauto using NoDup; rewrite PS.add_spec;
-        rewrite Hset; destruct 1; auto.
-  Qed.
+      destruct x1. apply assert_clock_spec in EQ1.
+      repeat split; eauto; try rewrite PS.add_spec, Hset;
+        try destruct 1; eauto using NoDup.
+    Qed.
 
   Lemma wt_elab_equation:
     forall aeq eq,
@@ -707,27 +631,28 @@ Section ElabExpressions.
       repeat progress
              match goal with
              | H:bind _ _ = _ |- _ => monadInv H
+             | H:bind2 _ _ = _ |- _ => monadInv H
              | H:elab_lexp _ = OK _ |- _ => apply wt_elab_lexp in H
-             | H:elab_lexps _ _ _ = OK _ |- _ => apply wt_elab_lexps in H
+             | H:elab_lexps _ _ _ _ = OK _ |- _ => apply wt_elab_lexps in H
              | H:find_clock _ _ = OK _ |- _ => apply wt_find_clock in H
              | H:find_type _ _ = OK _ |- _ => apply find_type_In in H
              | H:assert_type _ _ _ = OK _ |- _ => apply assert_type_In in H
              | H:elab_cexp _ = OK _ |- _ => apply wt_elab_cexp in H
              | H:_ ==b _ = true |- _ => rewrite equiv_decb_equiv in H
-             | H:check_result_list _ _ _ = OK ?x |- _ =>
+             | H:check_result_list _ _ _ _ = OK ?x |- _ =>
                apply check_result_list_Forall2 in H;
-                 destruct H as (Hele & Hins & Hnodup)
+                 destruct H as (Hele & Hins & Hnodup & Hcks)
              | _ => NamedDestructCases
-             end; auto with dftyping.
-    - unfold find_type_unop in EQ4. NamedDestructCases.
+             end; intros; subst; auto with dftyping.
+    - unfold find_type_unop in EQ3. NamedDestructCases.
       rewrite type_unop'_correct in Heq1.
       auto with dftyping.
-    - unfold find_type_binop in EQ6. NamedDestructCases.
-      rewrite type_binop'_correct in Heq1.
+    - unfold find_type_binop in EQ5. NamedDestructCases.
+      rewrite type_binop'_correct in Heq2.
       auto with dftyping.
     - apply andb_prop in Heq.
-      destruct Heq as (Heq2 & Heq3).
-      rewrite equiv_decb_equiv in Heq2, Heq3.
+      destruct Heq as (Heq4 & Heq5).
+      rewrite equiv_decb_equiv in Heq4, Heq5.
       auto with dftyping.
     - auto using type_castop with dftyping.
     - rename x1 into xin, x2 into xout, x3 into ein, xs into sxs, l0 into xs,
@@ -761,18 +686,43 @@ Section ElabExpressions.
       repeat progress
              match goal with
              | H:bind _ _ = _ |- _ => monadInv H
+             | H:bind2 _ _ = _ |- _ => monadInv H
+             | H:elab_lexp _ = OK _ |- _ => apply wc_elab_lexp in H
+             | H:elab_lexps _ _ _ _ = OK _ |- _ => apply wc_elab_lexps in H
+             | H:find_clock _ _ = OK _ |- _ => apply find_clock_clk_var in H
+             | H:elab_cexp _ = OK _ |- _ => apply wc_elab_cexp in H
              | H:_ ==b _ = true |- _ => rewrite equiv_decb_equiv in H
              | H:equiv _ _ |- _ => rewrite <-H in *; clear H
-             | H:clock_of_cexp _ _ = OK _ |- _ => apply clock_of_cexp_spec in H
-             | H:clock_of_lexp _ _ = OK ?x |- _ =>
-               destruct x; apply clock_of_lexp_spec in H
-             | H:find_clock _ _ = OK _ |- _ => apply find_clock_clk_var in H
-             | H:assert_lexp_clocks _ _ _ = OK ?x |- _ =>
-               destruct x; apply assert_lexp_clocks_spec in H
-             | H:assert_clocks _ _ _ = OK ?x |- _ =>
-               destruct x; apply assert_clocks_spec in H
+             | H:equiv _ _ |- _ => rewrite H in *; clear H
+             | H:check_result_list _ _ _ _ = OK ?x |- _ =>
+               apply check_result_list_Forall2 in H;
+                 destruct H as (Hele & Hins & Hnodup & Hcks)
              | _ => NamedDestructCases
-             end; auto using Well_clocked_eq, clk_cexp, clk_lexp.
+             end; intros; subst;
+        auto using Well_clocked_eq, clk_cexp, clk_lexp with dftyping.
+  Qed.
+
+  Fixpoint check_clock (loc: astloc) (ck: clock) : res unit :=
+    match ck with
+    | Cbase => OK tt
+    | Con ck x b =>
+      do ok <- check_clock loc ck;
+      do xck <- find_clock loc x;
+      if xck ==b ck then OK tt
+      else Error (err_loc loc ((MSG "badly-formed clock "
+                                    :: msg_of_clocks xck ck)))
+    end.
+  
+  Lemma check_clock_spec:
+    forall loc ck,
+      check_clock loc ck = OK tt ->
+      clk_clock cenv ck.
+  Proof.
+    induction ck; simpl; intro HH; auto using clk_clock.
+    monadInv HH; NamedDestructCases.
+    apply find_clock_clk_var in EQ1.
+    rewrite equiv_decb_equiv in Heq. rewrite Heq in *.
+    destruct x. auto.
   Qed.
 
 End ElabExpressions.
